Improve tail-call/guard-elimination of simple "oc" function
Previously, the version that was supposedly oblivious to the
precondition snuck in a dependency to that precondition via its
apply_kont function. And thus, various "CV-translatable" claims were
bogus.

I think the situation is improved now, but I still have to actually do
unify.

examples/algorithms/unification/triangular/first-order/tcallUnifScript.sml
@@ -127,7 +127,7 @@ Definition dfkwalkstar_def:
 End
 
 
-(* CV-translatable *)
+(* CV-translatable if dfkwalkstar is, which it isn't *)
 Theorem apply_kw_thm =
         SRULE [GSYM dfkwalkstar_def] $
               LIST_CONJ [cj 1 apply_kw_def,
@@ -140,53 +140,6 @@ Theorem dfkwalkstar_thm =
           |> SPEC_ALL
           |> ONCE_REWRITE_RULE [kwalkstar_thm]
           |> SRULE[GSYM apply_kw_thm, SF ETA_ss, GSYM dfkwalkstar_def]
-
-Definition core_dfkwalkstar_def:
-  core_dfkwalkstar s t0 k0 =
-  WHILE (λ(t, k). ispair t)
-        (λ(t, k). let (t1,t2) = destpair t
-                  in
-                    (walk_alt s t1, kwc2 t2 k))
-        (t0, k0)
-End
-
-(* CV-translatable *)
-Theorem core_dfkwalkstar_thm:
-  core_dfkwalkstar s t0 k0 =
-  case t0 of
-    Const cn => (t0, k0)
-  | Var n => (t0, k0)
-  | Pair t1 t2 => core_dfkwalkstar s (walk_alt s t1) (kwc2 t2 k0)
-Proof
-  simp[SimpLHS, Once whileTheory.WHILE, core_dfkwalkstar_def] >>
-  Cases_on ‘t0’ >> simp[core_dfkwalkstar_def]
-QED
-
-(* CV-translatable *)
-Definition dfkwalkstar_alt_def:
-  dfkwalkstar_alt s t0 k0 =
-  let t1 = walk_alt s t0 ;
-      (t, k) = core_dfkwalkstar s t1 k0
-  in
-    apply_kw s k t
-End
-
-Theorem dfkwalkstar_alt_correct:
-  wfs s ⇒ dfkwalkstar s t k = dfkwalkstar_alt s t k
-Proof
-  strip_tac >> map_every qid_spec_tac [‘k’, ‘t’] >>
-  ho_match_mp_tac walkstar_ind >> rpt strip_tac >>
-  simp[dfkwalkstar_alt_def] >> Cases_on ‘walk_alt s t’ >>
-  simp[Once dfkwalkstar_thm, Once core_dfkwalkstar_thm] >>
-  gvs[walk_alt_correct] >> simp[dfkwalkstar_alt_def]
-QED
-
-Theorem dfkwalkstar_alt_walkstar:
-  wfs s ⇒ walk* s t = dfkwalkstar_alt s t kwcID
-Proof
-  simp[GSYM dfkwalkstar_alt_correct, dfkwalkstar_def, kwalkstar_def, cwc_def,
-       apply_kw_thm]
-QED
 
 Definition koc_def:
   koc (s:α subst) t v k = cwc (oc s t v) k
@@ -206,6 +159,7 @@ Theorem koc_thm =
           |> SRULE [GSYM koc_def]
           |> SRULE [cwc_def, walk_alt_correctD]
 
+(* isomorphic to a list of terms *)
 Datatype: ockont = ocIDk | ock1 ('a term) ockont
 End
 
@@ -242,52 +196,181 @@ Theorem dfkoc_thm =
           |> ONCE_REWRITE_RULE [koc_thm]
           |> SRULE[GSYM apply_ockont_thm, SF ETA_ss, GSYM dfkoc_def]
 
-Definition core_oc_def:
-  core_oc s t k =
-  WHILE (λ(t,k). ispair t)
-        (λ(t,k). let (t1, t2) = destpair t in
-                   (walk_alt s t1, ock1 t2 k))
-        (t, k)
+(* INL is dfkoc; INR = apply_ockont *)
+Definition jointoc_def:
+  jointoc v (s, INL (t,k)) = dfkoc s t v k /\
+  jointoc v (s, INR (k,b)) = apply_ockont s v k b
 End
 
-(* CV-translatable *)
-Theorem core_oc_thm:
-  core_oc s t k =
-  case t of
-    Pair t1 t2 => core_oc s (walk_alt s t1) (ock1 t2 k)
-  | _ => (t, k)
+Theorem jointoc_thm = jointoc_def |> SPEC_ALL |> SRULE [Once dfkoc_thm]
+                                  |> SRULE [GSYM jointoc_def]
+
+val oc_code = rand “
+               tcall (K F)
+          [
+            INR ((λ(_,s). case s of INR (k,b) => b | _ => F),
+                 (λ(_,s). case s of INR (k,b) => b));
+            INR ((λ(_,s). ISR s /\ FST (OUTR s) = ocIDk),
+                 (λ(_,s). SND (OUTR s)));
+            INL (ISL o SND,
+                 (λ(s,sm).
+                    case sm of
+                      INL (t,k) =>
+                        (case walk_alt s t of
+                           Var n => (s,INR (k,v = n))
+                         | Pair t1 t2 => (s, INL (t1,ock1 t2 k))
+                         | Const cn => (s, INR (k,F)))));
+            INL (ISR o SND,
+                 (λ(s,sm). case sm of
+                           | INR (ock1 t k, b) => (s,INL (t,k))));
+          ]
+
+”
+
+Theorem jointoc_tcallish:
+  !x.
+    (λ(s,sm). wfs s) x ==>
+    jointoc v x =
+    tcall (K F) ^oc_code (jointoc v) x
 Proof
-  simp[SimpLHS, core_oc_def, Once whileTheory.WHILE] >>
-  Cases_on ‘t’ >> simp[core_oc_def]
+  simp[FUN_EQ_THM, sumTheory.FORALL_SUM, pairTheory.FORALL_PROD] >>
+  rw[jointoc_def]
+  >- (rename [‘walk_alt s t’] >> Cases_on ‘walk_alt s t’ >>
+      simp[jointoc_def] >> simp[Once dfkoc_thm]) >>
+  rename [‘apply_ockont s v k b’] >> Cases_on ‘k’ >>
+  simp[apply_ockont_thm, jointoc_def]
 QED
 
-(* CV-translatable *)
-Definition dfkoc_alt_def:
-  dfkoc_alt s t0 v k0 =
-  let t1 = walk_alt s t0 ;
-      (t, k) = core_oc s t1 k0 ;
-  in
-    case t of
-      Var u => apply_ockont s v k (v = u)
-    | Const _ => apply_ockont s v k F
-    | Pair _ _ => F
+Definition ocklist_def:
+  ocklist ocIDk = [] /\
+  ocklist (ock1 t k) = t::ocklist k
 End
 
-Theorem dfkoc_alt_correct:
-  wfs s ==> !t v k. dfkoc s t v k = dfkoc_alt s t v k
+Overload BAG_OF_LIST = “FOLDR BAG_INSERT EMPTY_BAG”
+
+Theorem FINITE_BAG_OF_LIST[simp]:
+  FINITE_BAG (BAG_OF_LIST l)
+Proof
+  Induct_on ‘l’ >> simp[]
+QED
+
+
+Definition BAG_OF_SUM[simp]:
+  BAG_OF_SUM (INL (t,k)) = BAG_OF_LIST (t :: ocklist k) /\
+  BAG_OF_SUM (INR (k,b)) = BAG_OF_LIST (ocklist k)
+End
+
+Definition ocR_def:
+  ocR (s:α subst) =
+  inv_image (pair$RPROD (=) (mlt1 (walkstarR s)) LEX $<)
+            (λ(s,sm). ((s,BAG_OF_SUM sm : α term bag),if ISR sm then 1 else 0))
+End
+
+Theorem WF_ocR:
+  wfs s ==> WF (ocR s)
+Proof
+  strip_tac >> simp[ocR_def] >>
+  irule relationTheory.WF_inv_image >>
+  irule pairTheory.WF_LEX >> simp[] >>
+  irule relationTheory.WF_SUBSET >>
+  simp[pairTheory.FORALL_PROD] >>
+  qexists ‘inv_image (mlt1 (walkstarR s)) SND’ >>
+  simp[walkstar_thWF, bagTheory.WF_mlt1, relationTheory.WF_inv_image,
+       pairTheory.PAIR_REL]
+QED
+
+Theorem mlt1_BAG_INSERT:
+  FINITE_BAG b ==> mlt1 R b (BAG_INSERT e b)
 Proof
   strip_tac >>
-  ho_match_mp_tac walkstar_ind >> rw[] >>
-  gvs[walk_alt_correct] >> simp[dfkoc_alt_def] >>
-  Cases_on ‘walk_alt s t’ >> gvs[] >>
-  simp[Once dfkoc_thm, Once core_oc_thm] >>
-  simp[dfkoc_alt_def]
+  simp[bagTheory.mlt1_def, bagTheory.BAG_INSERT_UNION] >>
+  simp[bagTheory.EL_BAG,
+       AC bagTheory.COMM_BAG_UNION bagTheory.ASSOC_BAG_UNION] >>
+  irule_at Any EQ_REFL >> qexists ‘EMPTY_BAG’ >> simp[]
+QED
+
+Theorem RTC_ocR_preserves_subst:
+  !x y. (ocR s0)^* (s1, x) (s2, y) ==> s1 = s2
+Proof
+  Induct_on ‘RTC’ >> simp[ocR_def, pairTheory.PAIR_REL] >>
+  simp[pairTheory.FORALL_PROD, pairTheory.LEX_DEF] >> metis_tac[]
+QED
+
+
+Theorem jointoc_cleaned0:
+  !x. (λ(s,sm). wfs s) x ==> jointoc v x = trec (K F) ^oc_code x
+Proof
+  match_mp_tac guard_elimination >> rpt conj_tac
+  >- (simp[pairTheory.FORALL_PROD, sumTheory.FORALL_SUM] >> rw[]
+      >- (rename [‘walk_alt s t’] >> Cases_on ‘walk_alt s t’ >> simp[]) >>
+      rename [‘k <> ocIDk’] >> Cases_on ‘k’ >> gs[])
+  >- (simp[pairTheory.FORALL_PROD] >> rw[] >>
+      rename [‘wfs th’] >>
+      qexists ‘ocR th’ >> simp[] >> conj_tac
+      >- (irule $ iffLR relationTheory.WF_EQ_WFP >> simp[WF_ocR]) >>
+      simp[sumTheory.FORALL_SUM, pairTheory.FORALL_PROD] >> rw[]
+      >- (rename [‘walk_alt s t’] >> Cases_on ‘walk_alt s t’ >>
+          simp[ocR0_def, ocR_def, ocklist_def, pairTheory.PAIR_REL,
+               pairTheory.LEX_DEF, mlt1_BAG_INSERT] >>
+          simp[bagTheory.mlt1_def] >>
+          rename [‘walk_alt s t = Pair t1 t2’] >>
+          qexistsl [‘t’, ‘{| t1; t2 |}’] >>
+          simp[bagTheory.BAG_UNION_INSERT] >>
+          simp[DISJ_IMP_THM, FORALL_AND_THM] >>
+          gs[GSYM walk_alt_correct] >>
+          dxrule_then strip_assume_tac RTC_ocR_preserves_subst >>
+          metis_tac[walkstar_th1, walkstar_th2]) >>
+      rename [‘k <> ocIDk’] >> Cases_on ‘k’ >> gvs[] >>
+      simp[ocR_def, ocklist_def, pairTheory.LEX_DEF]) >>
+  simp[sumTheory.FORALL_SUM, pairTheory.FORALL_PROD, jointoc_def] >>
+  rw[]
+  >- (rename [‘walk_alt s t’] >> Cases_on ‘walk_alt s t’ >>
+      simp[jointoc_def] >> simp[Once dfkoc_thm]) >>
+  rename [‘k <> ocIDk’] >> Cases_on ‘k’ >>
+  simp[apply_ockont_thm, jointoc_def]
+QED
+
+Definition dfkoc_alt_def:
+  dfkoc_alt s v t k = trec (K F) ^oc_code (s, INL (t,k))
+End
+
+Definition apply_kont'_def:
+  apply_kont' s v k b = trec (K F) ^oc_code (s, INR (k, b))
+End
+
+Theorem trec_term_case:
+  trec e opts (term_CASE t vf pf cf) =
+  case t of
+    Var v => trec e opts (vf v)
+  | Pair t1 t2 => trec e opts (pf t1 t2)
+  | Const cn => trec e opts (cf cn)
+Proof
+  Cases_on ‘t’ >> simp[]
+QED
+
+(* CV-translatable:
+     refers to itself, walk_alt and apply_kont'
+     apply_kont' refers to dfkoc_alt only
+*)
+Theorem dfkoc_alt_thm =
+        dfkoc_alt_def |> SRULE[Once trec_thm, tcall_EQN]
+                      |> SRULE [trec_term_case]
+                      |> SRULE[GSYM dfkoc_alt_def, GSYM apply_kont'_def]
+
+Theorem apply_kont'_thm:
+  apply_kont' s v ocIDk b = b /\
+  apply_kont' s v (ock1 t k) b = if b then T
+                                 else dfkoc_alt s v t k
+Proof
+  simp[apply_kont'_def] >> ONCE_REWRITE_TAC[trec_thm] >>
+  simp[tcall_EQN, GSYM dfkoc_alt_def]
 QED
 
 Theorem dfkoc_alt_oc:
-  wfs s ==> oc s t v = dfkoc_alt s t v ocIDk
+  wfs s ==> oc s t v = dfkoc_alt s v t ocIDk
 Proof
-  simp[GSYM dfkoc_alt_correct, dfkoc_def, koc_def, apply_ockont_def, cwc_def]
+  simp[dfkoc_alt_def, GSYM jointoc_cleaned0, jointoc_def, dfkoc_def,
+       koc_def, apply_ockont_def, cwc_def]
 QED
 
 Theorem contify_optbind:
@@ -305,9 +388,10 @@ Definition kunify_def:
 End
 
 Theorem disj_oc:
-  wfs s ==> (oc s t1 v \/ oc s t2 v <=> dfkoc_alt s t1 v (ock1 t2 ocIDk))
+  wfs s ==> (oc s t1 v \/ oc s t2 v <=> dfkoc_alt s v t1 (ock1 t2 ocIDk))
 Proof
-  simp[GSYM dfkoc_alt_correct, dfkoc_def, koc_def, cwc_def, apply_ockont_def]
+  simp[dfkoc_alt_def, GSYM jointoc_cleaned0, jointoc_def, dfkoc_def,
+       koc_def, cwc_def, apply_ockont_def]
 QED
 
 Theorem kunify_thm =
@@ -335,7 +419,7 @@ Definition apply_unifkont_def:
 End
 
 Definition dfkunify_def:
-  dfkunify A (s:α subst) t1 t2 k = kunify s t1 t2 (A k)
+  dfkunify (s:α subst) t1 t2 k = kunify s t1 t2 (apply_unifkont k)
 End
 
 Theorem apply_unifkont_thm =
@@ -349,7 +433,7 @@ Proof
 QED
 
 Theorem abs_EQ_apply_unifkont:
-  (λov. case ov of NONE => NONE | SOME s => dfkunify apply_unifkont s t1 t2 k) =
+  (λov. case ov of NONE => NONE | SOME s => dfkunify s t1 t2 k) =
   apply_unifkont (unifk1 t1 t2 k)
 Proof
   simp[FUN_EQ_THM, apply_unifkont_def, optionTheory.FORALL_OPTION, SF ETA_ss] >>
@@ -358,94 +442,20 @@ QED
 
 Theorem dfkunify_thm =
         dfkunify_def
-          |> Q.ISPEC ‘apply_unifkont’
           |> SPEC_ALL
           |> ONCE_REWRITE_RULE [kunify_thm]
           |> SRULE[GSYM dfkunify_def, apply_unifkont_NONE,
                    abs_EQ_apply_unifkont]
 
-Definition core_dfkunify_def:
-  core_dfkunify s t1 t2 k =
-  WHILE (λ(t1,t2,k). ispair t1 /\ ispair t2)
-        (λ(t1,t2,k).
-           let (t11,t12) = destpair t1 ;
-               (t21,t22) = destpair t2 ;
-           in
-             (walk_alt s t11,walk_alt s t21,unifk1 t12 t22 k))
-        (t1,t2,k)
-End
 
-(* CV-translatable *)
-Theorem core_dfkunify_thm:
-  core_dfkunify s t1 t2 k =
-  case (t1,t2) of
-    (Pair t11 t12, Pair t21 t22) =>
-      core_dfkunify s (walk_alt s t11) (walk_alt s t21) (unifk1 t12 t22 k)
-  | _ => (t1,t2,k)
-Proof
-  simp[SimpLHS, core_dfkunify_def, Once whileTheory.WHILE] >>
-  map_every Cases_on [‘t1’, ‘t2’] >> simp[] >>
-  simp[core_dfkunify_def]
-QED
 
-(* CV-translatable, once apply_unifkont is as well *)
-Definition dfkunify_alt_def:
-  dfkunify_alt A s t10 t20 k0 =
-  let t1 = walk_alt s t10 ; t2 = walk_alt s t20 ;
-      (T1,T2,k) = core_dfkunify s t1 t2 k0
-  in
-    case (T1,T2) of
-      (Var v1, Var v2) => if v1 = v2 then A k (SOME s)
-                          else A k (SOME (s |+ (v1,Var v2)))
-    | (Var v1, Const c2) => A k (SOME (s |+ (v1, Const c2)))
-    | (Var v1, Pair t1 t2) =>
-        if dfkoc_alt s t1 v1 (ock1 t2 ocIDk) then NONE
-        else A k (SOME (s |+ (v1, Pair t1 t2)))
-    | (Const c1, Var v2) => A k (SOME (s |+ (v2, Const c1)))
-    | (Const c1, Pair t1 t2) => NONE
-    | (Const c1, Const c2) => if c1 = c2 then A k (SOME s)
-                              else NONE
-    | (Pair t1 t2, Var v2) =>
-        if dfkoc_alt s t1 v2 (ock1 t2 ocIDk) then NONE
-        else A k (SOME (s |+ (v2, Pair t1 t2)))
-    | (Pair _ _, Pair _ _) => NONE
-    | (Pair t1 t2, Const c2) => NONE
-End
-
-Theorem dfkunify_alt_correct:
-  !s t1 t2 A k.
-    wfs s ==>
-    dfkunify apply_unifkont s t1 t2 k = dfkunify_alt apply_unifkont s t1 t2 k
-Proof
-  recInduct unify_ind >> rw[] >> gvs[walk_alt_correct] >>
-  simp[dfkunify_alt_def] >>
-  map_every Cases_on [‘walk_alt s t1’, ‘walk_alt s t2’] >> gvs[] >>
-  simp[Once dfkunify_thm, Once core_dfkunify_thm] >>
-  simp[dfkunify_alt_def]
-QED
-
+(*
 Theorem dfkunify_alt_unify:
   wfs s ==> unify s t1 t2 = dfkunify_alt apply_unifkont s t1 t2 unifIDk
 Proof
   simp[GSYM dfkunify_alt_correct, dfkunify_def, kunify_def, cwc_def,
        apply_unifkont_def]
 QED
-(*
-Definition apply_unifkont'_def:
-  apply_unifkont' unifIDk x = x /\
-  apply_unifkont' (unifk1 t1 t2 k) NONE = NONE /\
-  apply_unifkont' (unifk1 t1 t2 k) (SOME s) = dfkunify_alt s t1 t2 k
-End
-
-Theorem apply_unifkont'_rwt:
-  wfs s ==> apply_unifkont k (SOME s) = apply_unifkont' k (SOME s)
-Proof
-  Cases_on ‘k’ >>
-  simp[apply_unifkont'_def, apply_unifkont_thm, dfkunify_alt_correct]
-QED
-
-Theorem dfkunify_alt_thm = SRULE[apply_unifkont'_rwt] dfkunify_alt_def
 *)
-
 
 val _ = export_theory();
